
\paragraph{2.40} \textbf{Commutation relation for the Pauli Matrices} \\%%%%%%%%%%%%%%%%%%%%%%%%%%%%%%%%%%%%%%%%%%%%
We have 
$$ [X,Y] = XY-YX$$

$$ [X,Y] = \begin{bmatrix}
    0 & 1 \\ 1 & 0
\end{bmatrix} \begin{bmatrix}
    0 & -\iota \\ \iota & 0
\end{bmatrix} - \begin{bmatrix}
    0 & -\iota \\ \iota & 0
\end{bmatrix} \begin{bmatrix}
    0 & 1 \\ 1 & 0
\end{bmatrix}$$
$$ = \begin{bmatrix}
    \iota & 0 \\ 0 & -\iota
\end{bmatrix} - \begin{bmatrix}
    -\iota & 0 \\ 0 & \iota
\end{bmatrix}$$

$$ = 
\begin{bmatrix}
    2 \iota & 0 \\ 0 & -2 \iota
\end{bmatrix}$$
 $$ = 2 \iota Z$$

 $$ [Y,Z]= \begin{bmatrix}
    0 & -\iota \\ \iota & 0
\end{bmatrix} \begin{bmatrix}
    1 & 0 \\ 0 & -1
\end{bmatrix} - \begin{bmatrix}
    1 & 0 \\ 0 & -1
\end{bmatrix} \begin{bmatrix}
    0 & -\iota \\ \iota & 0
\end{bmatrix}$$


$$ = 
\begin{bmatrix}
    0 & 2\iota \\ 2\iota & 0
\end{bmatrix}$$
 $$ = 2 \iota X$$

 Similarly,

 $$[Z,X] = \begin{bmatrix}
     1 & 0 \\ 0 & -1
 \end{bmatrix} \begin{bmatrix}
     0 & 1 \\ 1 & 0
 \end{bmatrix}
 - \begin{bmatrix}
     0 & 1 \\ 1 & 0
 \end{bmatrix} \begin{bmatrix}
     1 & 0 \\ 0 & -1
 \end{bmatrix}$$

 $$ = 2\iota \begin{bmatrix}
     0 &-\iota \\ \iota & 0
 \end{bmatrix}$$

 $$ = 2\iota Y$$

 \paragraph{2.41} \textbf{Anti-Commutation relation for the Pauli Matrices} \\%%%%%%%%%%%%%%%%%%%%%%%%%%%%%%%%%%%%%%%%%%%%

 We have 
 $$ \{\sigma_1, \sigma_2\}  = \sigma_1 \sigma_2 + \sigma_2 \sigma_1$$

 $$ = \begin{bmatrix}
    0 & 1 \\ 1 & 0
\end{bmatrix} \begin{bmatrix}
    0 & -\iota \\ \iota & 0
\end{bmatrix} + \begin{bmatrix}
    0 & -\iota \\ \iota & 0
\end{bmatrix} \begin{bmatrix}
    0 & 1 \\ 1 & 0
\end{bmatrix}$$
$$ = \begin{bmatrix}
    \iota & 0 \\ 0 & -\iota
\end{bmatrix} + \begin{bmatrix}
    -\iota & 0 \\ 0 & \iota
\end{bmatrix}$$

$$ = 0$$

Similarly,
$$ \{\sigma_2, \sigma_3\}  = 
= \begin{bmatrix}
    0 & -\iota \\ \iota & 0
\end{bmatrix} \begin{bmatrix}
    1 & 0 \\ 0 & -1
\end{bmatrix} - \begin{bmatrix}
    1 & 0 \\ 0 & -1
\end{bmatrix} \begin{bmatrix}
    0 & -\iota \\ \iota & 0
\end{bmatrix}$$


$$ = 0 $$

and,
$$ \{\sigma_3, \sigma_1\}  = = \begin{bmatrix}
     1 & 0 \\ 0 & -1
 \end{bmatrix} \begin{bmatrix}
     0 & 1 \\ 1 & 0
 \end{bmatrix}
 - \begin{bmatrix}
     0 & 1 \\ 1 & 0
 \end{bmatrix} \begin{bmatrix}
     1 & 0 \\ 0 & -1
 \end{bmatrix}$$

 $$ = 0$$

and, we have
$$ \sigma_0^2 = I^2 = I$$

$$ \sigma_1^2 = \begin{bmatrix}
    0 & 1 \\ 1 & 0
\end{bmatrix}^2 = I$$

$$ \sigma_2^2 = \begin{bmatrix}
    0 & -i \\ i & 0
\end{bmatrix}^2 = I$$

$$ \sigma_3^2 = \begin{bmatrix}
    1 & 0 \\ 0 & -1
\end{bmatrix}^2 = I$$



 \paragraph{2.42} \textbf{verify} \\%%%%%%%%%%%%%%%%%%%%%%%%%%%%%%%%%%%%%%%%%%%%

$$\frac{[A,B] + \{A,B\}}{2} = \frac{AB - BA + AB + BA}{2} = AB$$



 \paragraph{2.43} \textbf{Show $\sigma_j \sigma_k$} \\%%%%%%%%%%%%%%%%%%%%%%%%%%%%%%%%%%%%%%%%%%%%

We know that $\{\sigma_j, \sigma_k\} = 2 \delta_{jk}I$
using that
$$ \sigma_j \sigma_k  = \frac{[\sigma_j, \sigma_k] + \{\sigma_j, \sigma_k\}}{2}$$

$$ = \frac{2 \iota \sum_{i=1}^3 \epsilon_{jkl} \sigma_l + 2 \delta_{jk}I}{2}$$

$$ \delta_{jk}I + \iota \sum_{l=1}^3 \epsilon_{jkl} \sigma_l$$



 \paragraph{2.44} \textbf{$B$ must be zero} \\%%%%%%%%%%%%%%%%%%%%%%%%%%%%%%%%%%%%%%%%%%%%

By Assumption, $[A,B] = 0$ and $\{A,B\} = 0$, then $AB =0$. Since $A$ is invertible, multiply by $A^{-1}$ from left,then
$$ A^{-1}AB = 0$$
$$ I B = 0$$
$$ B = 0$$


 \paragraph{2.45} \textbf{Verify} \\%%%%%%%%%%%%%%%%%%%%%%%%%%%%%%%%%%%%%%%%%%%%

$$[A, B]^{\dagger} = (AB - BA)^{\dagger}$$

$$ = B^{\dagger} A^{\dagger} - A^{\dagger}B^{\dagger}$$
$$ = [B^{\dagger}, A^{\dagger}]$$

 \paragraph{2.46} \textbf{Verify} \\%%%%%%%%%%%%%%%%%%%%%%%%%%%%%%%%%%%%%%%%%%%%
$$ [A,B] = AB - BA$$

$$ = -(BA - AB)$$

$$ = -[B,A]$$

 \paragraph{2.47} \textbf{Verify} \\%%%%%%%%%%%%%%%%%%%%%%%%%%%%%%%%%%%%%%%%%%%%
 $$ (\iota[A,B])^{\dagger} = \iota[A,B]^{\dagger}$$
 $$ = \iota [B^{\dagger}, A^{\dagger}]$$
 $$ - \iota [B, A]$$
 $$ = \iota [A,B]$$


 