\paragraph{2.54} \textbf{$\exp{A} \exp{B} = \exp{A + B}$}%%%%%%%%%%%%%%%%%%%%%%%%%%%%%%%%%%%%%%%%%%%%
\\
Since $[A,B] = 0$, $A$ and $B$ are simultaneously diagonlizable , $A = \sum_i a_i |i\rangle \langle i |$, and $B = \sum_i b_i |i\rangle \langle i |$.

So, 
$$ \exp{A} \exp{B} = \bigg( \sum_i \exp{a_i}|i\rangle \langle i |\bigg) \bigg( \exp{b_I} |i\rangle \langle i | $$

$$ = \sum_{i,j} \exp{a_i + b_j}|i\rangle \langle i | j\rangle \langle j | $$

$$ = \sum_{i,j} \exp{a_i + b_j}|i\rangle \langle j | \delta_{i,j}$$

$$ = \sum_{i} \exp{a_i + b_i}|i\rangle \langle i |$$

$$ \exp{A+B}$$

\paragraph{2.55} \textbf{$U(t_1, t_2)$ is unitary}%%%%%%%%%%%%%%%%%%%%%%%%%%%%%%%%%%%%%%%%%%%%
\\
$$ H = \sum_{E} E |E\rangle \langle E|$$

$$ U(t_2 - t_1) U^{\dagger} (t_2 - t_1) = \exp{\frac{-\iota H (t_2 - t_1)}{\hbar}} \exp{\frac{\iota H (t_2 - t_1)}{\hbar}} $$

$$ = \sum_{E,E'}\bigg(\exp{\frac{-\iota E (t_2 - t_1)}{\hbar}} |E\rangle \langle E|\bigg) \bigg(\exp{\frac{-\iota E' (t_2 - t_1)}{\hbar}} |E'\rangle \langle E'|\bigg) $$
$$ = \sum_E \exp{0} |E\rangle \langle E|$$

$$ \sum_E |E\rangle \langle E|$$
$$ = I$$

Similarly , $U^{\dagger}(t_2 - t_1)U(t_2 - t_1) = I$

\paragraph{2.56} \textbf{Spectral Decomposition}%%%%%%%%%%%%%%%%%%%%%%%%%%%%%%%%%%%%%%%%%%%%
\\
$$ U = \sum_i \lambda_i |\lambda_i \rangle \langle \lambda_i|$$
Now,
$$ \log(U) = \sum_{j} \log(\lambda_j) |\lambda_j \rangle \langle \lambda_j| = \sum_j \iota \theta_j |\lambda_j\rangle \langle \lambda_j|$$
where $\theta_j = \text{ arg }(\lambda_j)$
$$ K = \iota \log(U) = \sum_j \theta_j |\lambda_j\rangle \langle \lambda_j|$$

$$ K^{\dagger} =  (\iota \log U)^{\dagger}  = \bigg( \sum_j \theta_j |\lambda_j\rangle \langle \lambda_j| \bigg)^{\dagger} = \sum_j \theta_j |\lambda_j\rangle \langle \lambda_j| = K$$

\paragraph{2.57} \textbf{Cascaded Measurements are single measurements}%%%%%%%%%%%%%%%%%%%%%%%%%%%%%%%%%%%%%%%%%%%%
\\
We have 
$$ |\phi\rangle = \frac{ L_l |\psi\rangle}{\sqrt{\langle \psi| L_l^{\dagger } L_l | \psi\rangle}}$$

$$ \langle \phi| M_m^{\dagger} M_m|\phi \rangle = \frac{ \langle \psi| L_l^{\dagger }M_m^{\dagger} M_m L_l |\psi\rangle}{\langle \psi| L_l^{\dagger } L_l | \psi\rangle}$$

$$ \frac{M_m |\phi\rangle}{\sqrt{\langle \phi | M_m^{\dagger} M_m| \phi\rangle}} = \frac{M_m L_l |\phi\rangle}{\sqrt{\langle \phi |L_l^{\dagger} L_l| \phi\rangle}} = 
\frac{\sqrt{\langle \psi| L_l^{\dagger} L_l|\psi\rangle }}{\sqrt{\langle \psi |  L_l^{\dagger }M_m^{\dagger} M_m L_l |\psi\rangle}}$$

$$ = \frac{M_m L_l|\psi\rangle}{\sqrt{\langle \psi |  L_l^{\dagger }M_m^{\dagger} M_m L_l |\psi\rangle}}$$

$$ = \frac{N_{lm}|\psi\rangle}{\sqrt{\langle \psi | N_{lm}^{\dagger} N_{lm} |\psi\rangle}}$$
