
\paragraph{8.1}
The density operator of the initial state is written by $kb \psi$ and final form is written by $U kb \psi U^\dagger$.

Thus time development of $\rho = kb \psi$ can be written by 
$\mathcal{E}(\rho) = U\rho U^\dagger$.

\paragraph{8.2}
From eqn (2.147) (on page 100),
\begin{align*}
	\rho_m = \frac{M_m \rho M_m^\dagger}{\Tr (M_m^\dagger  M_m\rho ) }
					= \frac{M_m \rho M_m^\dagger}{\Tr ( M_m \rho M_m^\dagger ) }
					= \frac{\mathcal{E}_m (\rho)}{\Tr \mathcal{E}_m (\rho)}.
\end{align*}

And from eqn (2.143) (on page 99), $p(m) = Tr (M_m^\dagger M_m \rho) = Tr (M_m \rho M_m^\dagger) = Tr \mathcal {E}_m (\rho)$.

\paragraph{8.4}
First let's compute $U$
\begin{align*}
    U & = P_0 \otimes I + P_1 \otimes X\\
    & = \begin{bmatrix} I & 0 \\ 0 & X \end{bmatrix}\\
    & = \begin{bmatrix} 1 &0 & 0 & 0\\
    0 & 1 & 0 & 0\\
    0 & 0 & 0 & 1\\
    0 & 0 & 1 & 0
    \end{bmatrix}\\
    & = C_{NOT}
\end{align*}
Recall: Operator-sum representation is $\mathcal E(\rho) = \sum_k E_k \rho E_k^\dagger$, where $E_k = \braket{e_k | U | e_0}$.\\
Given in the problem prompt, the environment initializes in $\ket 0$
\begin{align*}
    \therefore \ket{e_0} = \ket 0
\end{align*}
Our final answer is:
\begin{align*}
    \boxed{\mathcal E(\rho) = \sum_k E_k \rho E_k^\dagger \  \text{ s.t. } \ E_k = \braket{e_k | C_{NOT} | 0}}
\end{align*}
